\documentclass[12pt]{article}
\begin{document}

Homework 3

Problem 2

Solution

a) Logistic Function

$ \sigma(\alpha) = \frac{1}{1+e^{(-\alpha)}}$

$ \sigma(\alpha) = \frac{e^\alpha}{1+e^\alpha}$

$= (e^\alpha){(1+e^\alpha)}^{-1}$

Chain Rule

$\frac{d\sigma}{d\alpha} = (e^\alpha){(1+e^\alpha)}^{-1} + (e^\alpha){(1+e^\alpha)}^{-2}(e^\alpha)$

$\frac{d\sigma}{d\alpha}= \frac{(e^\alpha)(1+e^\alpha)}{{(1+e^\alpha)^2}}- \frac{{e^\alpha}^2}{{(1+e^\alpha)^2}}$


$= \frac{(e^\alpha)}{{(1+e^\alpha)^2}}$

$ = \frac{(e^\alpha)}{(1+e^\alpha)} * \frac{1}{(1+e^\alpha)}$

$= \sigma(\alpha)*\sigma(-\alpha)$

$= \sigma(\alpha)(1-\sigma(\alpha))$

b)

Log function: 

$l(w) = \log \prod_{n=1}^N P(y_n|x_n)$

Re-writing the equation 

$l(w) = \prod_{n=1}^N P(y_n|x_n)$

Therefore

$P(y_n|x_n) = P(y_n = +1|x_n)*P(y_n = -1|x_n)$

$l(w) = \Sigma_{n=1}^N\log(P(y_n = +1|x_n) * P(y_n = +1|x_n))$

$l(w) = \Sigma_{n=1}^N\log(P(y_n = +1|x_n) * (1 - P(y_n = +1|x_n)))$

$l(w) = \Sigma_{n=1}^N([y_n = +1] \log P(y_n = +1|x_n)+[1 -(y_n = +1)]\log(1 - P(y_n = +1|x_n))$

$l(w) = \Sigma_{n=1}^N[[y_n = +1]\log(\frac{1}{1+e^{-w^{T}x_{n}y_{n}}})+[1 - (y_n = +1)]\log(\frac{e^{-w^{T}x_{n}y_{n}}}{{1+e^{-w^{T}x_{n}y_{n}}}})]$

$l(w) = \Sigma_{n=1}^N[-[y_n = +1]log(1+e^{-w^{T}x_{n}y_{n}})+ [1-(y_n = +1)]((-w^{T}x_{n}y_{n})-\log(1+e^{-w^{T}x_{n}y_{n}}))]$

$l(w) = \Sigma_{n=1}^N[-[1-(y_n = +1)](-w^{T}x_{n}y_{n})-\log(1+e^{-w^{T}x_{n}y_{n}})]$

Derivative W.r.t w:


$\frac{dl(w)}{dw} = \Sigma_{n=1}^N[-[1-(y_n = +1)]\frac{d}{dw}(-w^{T}x_{n}y_{n})-\frac{d}{dw}(1+e^{-w^{T}x_{n}y_{n}})]$

$\frac{dl(w)}{dw} =(x_ny_n)\Sigma_{n=1}^N[[1-(y_n = +1)]+P(y_n =-1|x_n)]$

$\frac{dl(w)}{dw} =(-x_ny_n)\Sigma_{n=1}^N[[(y_n = +1)]-P(y_n =-1|x_n)]$

After Averaging:

$\Delta_{w}l(w)= \frac{dl(w)}{dw} = \frac{1}{N}(-x_ny_n)\Sigma_{n=1}^N[[(y_n = +1)]-P(y_n =-1|x_n)]$

$\Delta_{w}l(w)= \frac{1}{N}(-x_ny_n)\Sigma_{n=1}^N\sigma(-y_nw^Tx_n)$

$\Delta_{w}l(w)= \frac{1}{N}(-y_nx_n)\Sigma_{n=1}^N\sigma(-y_nw^Tx_n)$


(c)


Taylor expression:

$\Delta_{w}l(w)=l(w)(w(0)+ \eta\upsilon)-l(w(0))$

$ = \eta\Deltal(w)(w(0))^T\upsilon + O(\eta)^2 $

$\geq-\eta||\Deltal(w)(w(0))^T||$

Deriving the update step

$e_n(w)=ln(1+e^{-y_nw^{T}I_n}$

$\Deltae_n(w)=\frac{-y_nx_n}{1+e^{y_nw^Tx_n}}$

Updated weight:

$w\leftarrow w-\eta\Deltae_n(w)$

Expected weight:

$ -\eta\frac{1}{N}\Sigma_{n=1}^N\Deltae_n(w)$


\end{document}